Started lazy evaluation (eval not complete yet!)

Evaluate.thy
@@ -1,20 +1,123 @@
-theory EvaluateEager
-imports EvaluationContext
+theory Evaluate
+imports Typecheck
 begin
 
-inductive reduce :: "expr \<Rightarrow> expr \<Rightarrow> bool" (infix "\<leadsto>\<^sub>\<beta>" 60) where
-  ev_beta [simp]: "is_value e\<^sub>2 \<Longrightarrow> App (Abs t e\<^sub>1) e\<^sub>2 \<leadsto>\<^sub>\<beta> subst\<^sub>e\<^sub>e 0 e\<^sub>2 e\<^sub>1" 
-| ev_let [simp]: "is_value e\<^sub>1 \<Longrightarrow> Let e\<^sub>1 e\<^sub>2 \<leadsto>\<^sub>\<beta> subst\<^sub>e\<^sub>e 0 e\<^sub>1 e\<^sub>2"
-| ev_proj [simp]: "is_value_f fs \<Longrightarrow> lookup l fs = Some e \<Longrightarrow> Proj (Rec fs) l \<leadsto>\<^sub>\<beta> e" 
-| ev_case [simp]: "is_value e \<Longrightarrow> lookup l cs = Some e' \<Longrightarrow> Case (Inj l ts e) t cs \<leadsto>\<^sub>\<beta> subst\<^sub>e\<^sub>e 0 e e'" 
-| ev_fold [simp]: "is_value e \<Longrightarrow> Unfold t (Fold t e) \<leadsto>\<^sub>\<beta> e" 
-| ev_tbeta [simp]: "TyApp (TyAbs k e) t \<leadsto>\<^sub>\<beta> subst\<^sub>t\<^sub>e 0 t e" 
-| ev_tlet [simp]: "TyLet t e \<leadsto>\<^sub>\<beta> subst\<^sub>t\<^sub>e 0 t e" 
-
 inductive evaluate :: "expr \<Rightarrow> expr \<Rightarrow> bool" (infix "\<leadsto>" 60) where
-  ev_stack [simp]: "unstack_eager e = (s, r) \<Longrightarrow> r \<leadsto>\<^sub>\<beta> r' \<Longrightarrow> e \<leadsto> restack s r'"
+  ev_app1 [simp]: "e\<^sub>1 \<leadsto> e\<^sub>1' \<Longrightarrow> App e\<^sub>1 e\<^sub>2 \<leadsto> App e\<^sub>1' e\<^sub>2" 
+| ev_app2 [simp]: "App (Abs t e\<^sub>1) e\<^sub>2 \<leadsto> Let e\<^sub>2 e\<^sub>1"
+| ev_let1 [simp]: "e\<^sub>2 \<leadsto> e\<^sub>2' \<Longrightarrow> Let e\<^sub>1 e\<^sub>2 \<leadsto> Let e\<^sub>1 e\<^sub>2'"
+| ev_rec [simp]: "list_all is_var vs \<Longrightarrow> \<not> is_var e \<Longrightarrow> 
+    Rec (vs @ [e] @ nvs) \<leadsto> Let e (Rec (map (incr\<^sub>e\<^sub>e 0) vs @ [Var 0] @ map (incr\<^sub>e\<^sub>e 0) nvs))" 
+| ev_proj1 [simp]: "e \<leadsto> e' \<Longrightarrow> Proj e l \<leadsto> Proj e' l"
+| ev_proj2 [simp]: "list_all is_var fs \<Longrightarrow> lookup l fs = Some e \<Longrightarrow> Proj (Rec fs) l \<leadsto> e" 
+| ev_inj [simp]: "\<not> is_var e \<Longrightarrow> Inj l ts e \<leadsto> Let e (Inj l ts (Var 0))"
+| ev_case1 [simp]: "e \<leadsto> e' \<Longrightarrow> Case e t cs \<leadsto> Case e' t cs"
+| ev_case2 [simp]: "is_var e \<Longrightarrow> lookup l cs = Some e' \<Longrightarrow> Case (Inj l ts e) t cs \<leadsto> subst\<^sub>e\<^sub>e 0 e e'"
+| ev_fold [simp]: "\<not> is_var e \<Longrightarrow> Fold t e \<leadsto> Let e (Fold t (Var 0))" 
+| ev_unfold1 [simp]: "e \<leadsto> e' \<Longrightarrow> Unfold t e \<leadsto> Unfold t e'"  
+| ev_unfold2 [simp]: "is_var e \<Longrightarrow> Unfold t (Fold t e) \<leadsto> e" 
+| ev_tyapp1 [simp]: "e \<leadsto> e' \<Longrightarrow> TyApp e t \<leadsto> TyApp e' t" 
+| ev_tyapp2 [simp]: "TyApp (TyAbs k e) t \<leadsto> subst\<^sub>t\<^sub>e 0 t e" 
+| ev_tylet [simp]: "TyLet t e \<leadsto> subst\<^sub>t\<^sub>e 0 t e" 
 
-inductive_cases [elim]: "e \<leadsto> e'"
+lemma [elim]: "e \<leadsto> e' \<Longrightarrow> is_value e \<Longrightarrow> False"
+  by (induction e e' rule: evaluate.induct) simp_all
+
+lemma [elim]: "e \<leadsto> e' \<Longrightarrow> is_var e \<Longrightarrow> False"
+  by (induction e e' rule: evaluate.induct) simp_all
+
+lemma [elim]: "list_all is_var vs \<Longrightarrow> list_all is_var vs' \<Longrightarrow> \<not> is_var e \<Longrightarrow> \<not> is_var e' \<Longrightarrow>
+    vs @ [e] @ nvs = vs' @ [e'] @ nvs' \<Longrightarrow> vs = vs'"
+  proof (induction vs arbitrary: vs')
+  case Nil
+    thus ?case by (induction vs') simp_all
+  next case (Cons v vs)
+    thus ?case by (induction vs') simp_all
+  qed
+
+theorem determinacy [elim]: "e \<leadsto> e' \<Longrightarrow> e \<leadsto> e'' \<Longrightarrow> e' = e''"
+  proof (induction e e' arbitrary: e'' rule: evaluate.induct)
+  case (ev_app1 e\<^sub>1 e\<^sub>1' e\<^sub>2)
+    with ev_app1(3) show ?case
+      proof (induction "App e\<^sub>1 e\<^sub>2" e'' rule: evaluate.induct)
+      case ev_app2
+        hence False by auto
+        thus ?case by simp
+      qed simp_all
+  next case (ev_app2 t e\<^sub>1 e\<^sub>2)
+    thus ?case by (induction "App (Abs t e\<^sub>1) e\<^sub>2" e'' rule: evaluate.induct) auto
+  next case (ev_let1 e\<^sub>2 e\<^sub>2' e\<^sub>1)
+    with ev_let1(3) show ?case by (induction "Let e\<^sub>1 e\<^sub>2" e'' rule: evaluate.induct) simp_all
+  next case (ev_rec vs e nvs)
+    with ev_rec(3) show ?case
+      proof (induction "Rec (vs @ [e] @ nvs)" e'' rule: evaluate.induct)
+      case (ev_rec vs' e\<^sub>2 nvs')
+        hence "vs' = vs" by auto
+        with ev_rec show ?case by simp
+      qed
+  next case (ev_proj1 e e' l)
+    with ev_proj1(3) show ?case
+      proof (induction "Proj e l" e'' rule: evaluate.induct)
+      case ev_proj2
+        hence False by auto
+        thus ?case by simp
+      qed simp_all
+  next case (ev_proj2 fs l e)
+    with ev_proj2(3) show ?case
+      proof (induction "Proj (Rec fs) l" e'' rule: evaluate.induct)
+      case ev_proj1
+        hence False by auto
+        thus ?case by simp
+      qed simp_all
+  next case (ev_inj e l ts)
+    with ev_inj(2) show ?case by (induction "Inj l ts e" e'' rule: evaluate.induct) simp_all
+  next case (ev_case1 e e' t cs)
+    with ev_case1(3) show ?case
+      proof (induction "Case e t cs" e'' rule: evaluate.induct)
+      case ev_case2
+        hence False by auto
+        thus ?case by simp
+      qed simp_all
+  next case (ev_case2 e l cs e' ts t)
+    with ev_case2(3) show ?case
+      proof (induction "Case (Inj l ts e) t cs" e'' rule: evaluate.induct)
+      case ev_case1
+        hence False by auto
+        thus ?case by simp
+      qed simp_all
+  next case (ev_fold e t)
+    with ev_fold(2) show ?case by (induction "Fold t e" e'' rule: evaluate.induct) simp_all
+  next case (ev_unfold1 e e' t)
+    with ev_unfold1(3) show ?case
+      proof (induction "Unfold t e" e'' rule: evaluate.induct)
+      case ev_unfold2
+        hence False by auto
+        thus ?case by simp
+      qed simp_all
+  next case (ev_unfold2 e t)
+    with ev_unfold2(2) show ?case
+      proof (induction "Unfold t (Fold t e)" e'' rule: evaluate.induct)
+      case ev_unfold1
+        hence False by auto
+        thus ?case by simp
+      qed simp_all
+  next case (ev_tyapp1 e e' t)
+    with ev_tyapp1(3) show ?case
+      proof (induction "TyApp e t" e'' rule: evaluate.induct)
+      case ev_tyapp2
+        hence False by auto
+        thus ?case by simp
+      qed simp_all
+  next case (ev_tyapp2 k e t)
+    thus ?case
+      proof (induction "TyApp (TyAbs k e) t" e'' rule: evaluate.induct)
+      case ev_tyapp1
+        hence False by auto
+        thus ?case by simp
+      qed simp_all
+  next case (ev_tylet t e)
+    thus ?case by (induction "TyLet t e" e'' rule: evaluate.induct) simp_all
+  qed
 
 theorem [simp]: "\<Delta>,[] \<turnstile> e : t \<Longrightarrow> unstack_eager e = (s, r) \<Longrightarrow> is_value e \<or> (\<exists>r'. r \<leadsto>\<^sub>\<beta> r')"
     and "\<Delta>,[] \<turnstile>\<^sub>f fs : ts \<Longrightarrow> \<not> is_value_f fs \<Longrightarrow> unstack_eager_f fs = (vs, nvs, s, r) \<Longrightarrow> \<exists>r'. r \<leadsto>\<^sub>\<beta> r'"
